popl17/UPGRADE.md
@@ -1,7 +1,7 @@
 Upgrade Guide
 ----------------------------
 
-This `popl17` directory contains many coq proof files written in coq 8.4. Could you upgrade their syntax to be compatible with coq 8.18? Do not touch other directories
+This `popl17` directory contains many coq proof files written in coq 8.4. Could you upgrade their syntax to be compatible with coq 8.18? Do not touch other directories.
 
 The structure of the project is written in `./AGENT.md`
 
